tests/lean/run/autoattachleak.lean
@@ -1,5 +1,18 @@
 /-! This tests demonstrates where and how auto-attaching leaks to the user -/
 
+-- Until stage0 update
+attribute [auto_attach]
+  List.map_wfParam
+  List.map_unattach
+  List.filter_wfParam
+  List.filter_unattach
+  List.reverse_wfParam
+  List.reverse_unattach
+  List.foldl_wfParam
+  List.foldl_unattach
+  Array.map_wfParam
+  Array.map_unattach
+
 structure Tree (α : Type) where
   cs : List (Tree α)
 
